Behavior proof WIP

theories/Dynamics/Procedure.v
@@ -1,10 +1,10 @@
-From stdpp Require Import base list.
+From stdpp Require Import base list stringmap gmap fin_maps.
 From Metaconfigurations.Syntax Require Import Value Term Stmt.
 
 From Metaconfigurations Require Import 
-  Map Syntax.Term Syntax.Stmt Syntax.Ty 
-  Syntax.Value Statics.Value 
-  Dynamics.Term Object Process.
+  Map Syntax.Term Syntax.Stmt
+  Syntax.Value
+  Dynamics.Term Object.
 From stdpp Require Import base.
 Require Import Coq.ZArith.BinInt.
 
@@ -14,7 +14,7 @@ From Metaconfigurations.Dynamics Require Import Term Stmt.
 Section Procedure.
   Variable Π : Type.
 
-  Context `{Process Π}.
+  Context `{Countable Π}.
 
   (* Type of implemented object *)
   Variable Ω₀ : Type.
@@ -31,79 +31,278 @@ Section Procedure.
 
   Context `{Object Π Ω}.
 
-  Definition procedure (π : Π) := list (Stmt.t Ω π).
+  Record procedure := {
+    param : string;
+    body : list (Stmt.t Π Ω);
+  }.
 
   Record Implementation := 
   {
     (* Initial states for every base object *)
-    inital_states : states;
+    initial_states : states Π Ω;
     (* Assignment from every process π and operation OP to a procedure *)
-    procedures π op : V⟦ (type ω).(ARG Π) op ⟧ → procedure π;
+    procedures : (type ω).(OP Π) → procedure;
   }.
 
-  Variant control :=
-    | Next (l : nat) 
-    | Return (v : Value.t)
-
-  Record frame π := {
+  Record frame := {
     pc : nat;
-    proc : procedure π;
+    registers : stringmap Value.t;
+    proc : procedure;
   }.
+
+  Variant signal :=
+    | Next (f : frame) (* On next step, go to line [l] *)
+    | Return (v : Value.t) (* Procedure has returned with value [v] *).
+
+  Variant step_procedure (π : Π) : states Π Ω → frame → states Π Ω → signal → Prop :=
+    | step_next pc pc' s ψ ψ' proc ϵ ϵ' :
+      (* If [pc] points to line containing statement [s] in [proc] *)
+      proc.(body) !! pc = Some s →
+      Stmt.eval π ψ ϵ s ψ' ϵ' (Goto pc') →
+      step_procedure π ϵ {| pc := pc; registers := ψ; proc := proc |} ϵ' (Next {| pc := pc'; registers := ψ'; proc := proc |})
+    | step_implicit_return pc ψ proc ϵ :
+      (* Control has fallen off end of procedure *)
+      proc.(body) !! pc = None →
+      step_procedure π ϵ {| pc := pc; registers := ψ; proc := proc |} ϵ (Return ⊤ᵥ)
+    | step_return pc s ψ proc ϵ ϵ' v:
+      proc.(body) !! pc = Some s →
+      Stmt.eval π ψ ϵ s ψ ϵ' (Stmt.Return v) →
+      step_procedure π ϵ {| pc := pc; registers := ψ; proc := proc |} ϵ (Return v).
 
   Record configuration := {
-    outstanding π : option (frame π);
-    ψ π : RegisterFile.t π;
-    ϵ : states;
+    outstanding : gmap Π frame;
+    ϵ : states Π Ω;
   }.
+
+  Variant line :=
+    | Invoke (op : (type ω).(OP Π)) (arg : Value.t)
+    | Intermediate
+    | Response (resp : Value.t).
+
+  Inductive run :=
+    | Initial (c : configuration)
+    | Step (r : run) (π : Π) (l : line) (c : configuration).
 
   Section Run.
 
     Variable impl : Implementation.
 
-    Variant line (π : Π) :=
-      | Invoke (op : (type ω).(OP Π)) (arg : Value.t)
-      | Intermediate
-      | Response (resp : Value.t).
+    Definition initial_frame op arg :=
+      let proc := procedures impl op in
+      {|
+        pc := 0;
+        registers := singletonM proc.(param) arg;
+        proc := proc;
+      |}.
 
-    Local Open Scope stmt_scope.
-
-    Inductive step : configuration → ∀ π : Π, line π → configuration → Prop :=
-    | step_intermediate c π c' s ψ' ϵ' pc pc' (proc : procedure π) :
+    Variant step : configuration → Π → line → configuration → Prop :=
+      | step_invoke outstanding π ϵ ϵ' op arg f :
+        outstanding !! π = None →
+        step_procedure π ϵ (initial_frame op arg) ϵ' (Next f) →
+        step {| outstanding := outstanding; ϵ := ϵ |} π (Invoke op arg) {| outstanding := <[π := f]>outstanding; ϵ := ϵ' |}
+      | step_intermediate outstanding π ϵ ϵ' f f' :
       (* If process [π] has an outstanding request for proecedure [proc], interrupted at line [pc] *)
-      c.(outstanding) π = Some {| pc := pc; proc := proc |} →
-      (* And [pc] points to line containing statement [s] in [proc] *)
-      proc !! pc = Some s →
-      (* And *)
-      Stmt.eval (c.(ψ) π) c.(ϵ) s ψ' ϵ' (Goto pc') →
-      step c π Intermediate {| outstanding |}
-      (⟨ ψ , ϵ , s ⟩ ⇓ₛ ⟨ ψ' , ϵ' , sig ⟩)%stmt_scope →
-      (⟨ (c.(ψ) π) , (c.(ϵ)) , s ⟩ ⇓ₛ ⟨ Ψ' , ϵ' , sig ⟩)%stmt_scope →
-      step c π c'
-      impl.(procedures) π !! c.(pc) π = Some l → step.
-      
-      Stmt.eval (c.(ψ) π) (c.(arg) pi c.(ϵ) l ψ ϵ → step .
+        outstanding !! π = Some f →
+        step_procedure π ϵ f ϵ' (Next f') →
+        step {| outstanding := outstanding; ϵ := ϵ |} π Intermediate {| outstanding := <[π := f']>outstanding; ϵ := ϵ' |}
+      | step_response outstanding π ϵ ϵ' f v :
+      (* If process [π] has an outstanding request for proecedure [proc], interrupted at line [pc] *)
+        outstanding !! π = Some f →
+        step_procedure π ϵ f ϵ' (Return v) →
+        step {| outstanding := outstanding; ϵ := ϵ |} π (Response v) {| outstanding := delete π outstanding; ϵ := ϵ' |}.
+
+    Definition final r :=
+      match r with
+      | Initial c | Step _ _ _ c => c
+      end.
+
+    Inductive Run : run → Prop :=
+      | Run_initial :  Run (Initial {| outstanding := ∅; ϵ := impl.(initial_states) |})
+      | Run_step r π l c : Run r → step (final r) π l c → Run (Step r π l c).
+
+    Fixpoint behavior r : list (Π * line) :=
+      match r with
+      | Initial _ => []
+      | Step r π l c =>
+          match l with
+          | Invoke _ _ | Response _ => behavior r ++ [(π, l)]
+          | Intermediate => behavior r
+          end
+      end.
+
+    Variant Behavior : list (Π * line) → Prop :=
+      | Behavior_intro (r : run) : Run r → Behavior (behavior r).
+
+    Lemma behavior_no_intermediate π l r : Behavior r → (π, l) ∈ r → l ≠ Intermediate.
+    Proof.
+    Admitted.
 
   End Run.
 
-  Inductive run :=
-    | Initial (c : configuration)
-    | Step (r : run) (π : Π) (c : configuration).
+End Procedure.
 
-  Definition final r :=
-    match r with
-    | Initial c | Step _ _ c => c
+Section Augmentation.
+
+  Variable Π : Type.
+
+  Context `{Countable Π}.
+
+  (* Type of implemented object *)
+  Variable Ω₀ : Type.
+
+  (* The object being implemented *)
+  Variable ω : Ω₀.
+
+  Context `{Object Π Ω₀}.
+
+  (* Set of base objects *)
+  Variable Ω : Type.
+
+  Context `{Object Π Ω}.
+
+  (* Auxillary objects *)
+  Variable Ω' : Type.
+
+  Context `{Object Π Ω'}.
+
+  (* Definition lift_term (e : Term.t Π Ω) :  Term.t Π (Ω + Ω').
+  Proof.
+  Defined. *)
+
+  Fixpoint lift_term (e : Term.t Π Ω) : Term.t Π (Ω + Ω') :=
+    match e with
+    | Var x => Var x
+    | Term.Invoke ω op arg => Term.Invoke (inl ω) op (lift_term arg)
+    | Bop op e₁ e₂ => Bop op (lift_term e₁) (lift_term e₂)
+    | Uop op e => Uop op (lift_term e)
+    | Term.Pair e₁ e₂ => Term.Pair (lift_term e₁) (lift_term e₂)
+    | ProjL e => ProjL (lift_term e)
+    | ProjR e => ProjR (lift_term e)
+    | Term.Int n => Term.Int n
+    | Term.Bool b => Term.Bool b
+    | Term.Unit => Term.Unit
     end.
 
-  Inductive step : configuration → Π → configuration → Prop :=
-    | step_intro c π c' :
+  Lemma lift_term_complete :
+    ∀ e π ψ (ϵ₁ ϵ₁' : states Π Ω) v (ϵ₂ : states Π Ω'),
+      Term.eval π ψ ϵ₁ e ϵ₁' v →
+        Term.eval π ψ (disjoint_union ϵ₁ ϵ₂) (lift_term e) (disjoint_union ϵ₁' ϵ₂) v.
+  Proof.
+    induction e; intros; simpl in *; inv H3; try (econstructor; eauto).
+    rewrite rebind_union_distr. econstructor.
+      + eapply IHe. eauto.
+      + inv H10. econstructor. unfold Map.lookup in *. simpl in *. assumption.
+  Qed.
 
-      Stmt.eval (c.(registers) π) c.(arg) (c.(pc) π)
-     
+  Lemma lift_term_sound_l :
+    ∀ e π ψ ϵ v ϵ',
+      Term.eval π ψ ϵ (lift_term e) ϵ' v →
+        Term.eval π ψ (πₗ ϵ) e (πₗ ϵ') v.
+  Proof.
+    induction e; intros; simpl in *; inv H3; try (econstructor; eauto).
+    rewrite πₗ_rebind_comm. econstructor.
+    + apply IHe. eassumption.
+    + inv H10. constructor. simpl in *.
+      replace (Map.lookup ω0 (πₗ ϵ0)) 
+          with (Map.lookup (inl ω0) ϵ0) by reflexivity.
+      assumption.
+  Qed.
 
-  Inductive run_wf : run → Prop :=
-    | Initial_wf c : run_wf (Initial c)
-    | Step_wf r π c : run_wf r →
+  Lemma lift_term_sound_r :
+    ∀ e π ψ ϵ v ϵ',
+      Term.eval π ψ ϵ (lift_term e) ϵ' v → πᵣ ϵ = πᵣ ϵ'.
+  Proof.
+    induction e; intros; simpl in *; inv H3; intuition.
+    - apply IHe in H9. subst. simpl in *.
+      replace (πᵣ ϵ0) with (πᵣ ϵ'0). apply rebind_l_πᵣ.
+    - apply IHe1 in H7. apply IHe2 in H10. congruence.
+    - inv H9. eauto.
+    - apply IHe1 in H6. apply IHe2 in H9. congruence.
+    - apply IHe in H5. assumption.
+    - apply IHe in H5. assumption.
+  Qed.
 
-  Reserved Notation "⟨ Ψ , ϵ , Φ , pc ⟩ ⇓ₛ ⟨ Ψ' , ϵ' , sig ⟩" (at level 80, no associativity).
+  Fixpoint lift_stmt (s : Stmt.t Π Ω) : Stmt.t Π (Ω + Ω') :=
+    match s with
+    | Seq s₁ s₂ => Seq (lift_stmt s₁) (lift_stmt s₂)
+    | Assign x e => Assign x (lift_term e)
+    | If e s₁ s₂ => If (lift_term e) (lift_stmt s₁) (lift_stmt s₂)
+    | Syntax.Stmt.Goto l => Syntax.Stmt.Goto l
+    | Syntax.Stmt.Return e => Syntax.Stmt.Return (lift_term e)
+    | Stmt.Invoke (Invocation ω op arg) => @Syntax.Stmt.Invoke _ (Ω + Ω') _ _ (Invocation (inl ω) op (lift_term arg))
+    | Skip => Skip
+    end.
 
-End Procedure.
+  Lemma lift_stmt_complete :
+    ∀ s π ψ ψ' (ϵ₁ ϵ₁' : states Π Ω) sig,
+      Stmt.eval π ψ ϵ₁ s ψ' ϵ₁' sig →
+        ∀ ϵ₂,
+          Stmt.eval π ψ (disjoint_union ϵ₁ ϵ₂) (lift_stmt s) ψ' (disjoint_union ϵ₁' ϵ₂) sig.
+  Proof.
+    intros. generalize dependent ϵ₂. induction H3; intros.
+    - econstructor.
+    - econstructor. fold lift_stmt. eauto.
+    - econstructor. eauto.
+    - econstructor; fold lift_stmt; eauto.
+    - econstructor; eauto. eapply lift_term_complete. auto.
+    - eapply eval_if_false.
+      + eapply lift_term_complete. eauto.
+      + fold lift_stmt. eapply IHeval.
+    - econstructor. eapply lift_term_complete. eassumption.
+    - econstructor.
+    - econstructor. eapply lift_term_complete in H3. eauto.
+    - econstructor. eapply lift_term_complete. eassumption.
+  Qed.
+
+  Lemma lift_stmt_sound_l :
+    ∀ s π ψ ϵ sig ψ' ϵ',
+      Stmt.eval π ψ ϵ (lift_stmt s) ψ' ϵ' sig →
+        Stmt.eval π ψ (πₗ ϵ) s ψ' (πₗ ϵ') sig.
+  Proof.
+    induction s; intros.
+    - inv H3; econstructor; eauto.
+    - inv H3. econstructor. eapply lift_term_sound_l. eassumption.
+    - inv H3.
+      + econstructor.
+        * eapply lift_term_sound_l. eassumption.
+        * eauto.
+      + eapply eval_if_false.
+        * eapply lift_term_sound_l. eassumption.
+        * eauto.
+    - inv H3. econstructor.
+    - inv H3. econstructor. eapply lift_term_sound_l. assumption.
+    - simpl in *. destruct inv. inv H3. econstructor. eapply lift_term_sound_l. simpl. eassumption.
+    - inv H3. econstructor.
+  Qed.
+
+  Lemma lift_stmt_sound_r :
+    ∀ s π ψ ϵ sig ψ' ϵ',
+      Stmt.eval π ψ ϵ (lift_stmt s) ψ' ϵ' sig → πᵣ ϵ = πᵣ ϵ'.
+  Proof.
+    induction s; intros.
+    - inv H3.
+      + eauto.
+      + eauto.
+      + etransitivity.
+        * eapply IHs1. eauto.
+        * eauto.
+    - inv H3. reflexivity.
+    - inv H3.
+      + etransitivity.
+        * eapply lift_term_sound_r. eassumption.
+        * eauto.
+      + etransitivity.
+        * eapply lift_term_sound_r. eassumption.
+        * eauto.
+    - inv H3. econstructor.
+    - inv H3. eapply lift_term_sound_r. eassumption.
+    - cbn in *. destruct inv. inv H3. eapply lift_term_sound_r.
+      assert (Term.Invoke (inl ω0) op (lift_term arg) = lift_term (Term.Invoke ω0 op arg)) by reflexivity.
+      erewrite <- H3.
+      eassumption.
+    - inv H3. econstructor.
+  Qed.
+
+  Definition augmentation : Stmt.t Π Ω
+  
+End Augmentation.
