theories/Dynamics/Stmt.v
@@ -1,15 +1,12 @@
 From Metaconfigurations Require Import 
-  Map Syntax.Term Syntax.Stmt Syntax.Ty 
-  Syntax.Value Statics.Value 
-  Dynamics.Term Object Process.
-From stdpp Require Import base.
+  Map Syntax.Term Syntax.Stmt
+  Syntax.Value Dynamics.Term Object.
+From stdpp Require Import base stringmap.
 Require Import Coq.ZArith.BinInt.
 
 Section Eval.
 
-  Context {Π : Type} `{Process Π}.
-
-  Variable Ω : Type.
+  Context {Π Ω : Type}.
 
   Context `{Object Π Ω}.
 
@@ -20,39 +17,40 @@ Section Eval.
     | Goto (l : nat)
     | Return (v : Value.t).
 
-  Reserved Notation "⧼ Ψ , ϵ , s ⧽ ⇓ₛ ⧼ Ψ' , ϵ' , sig ⧽" (at level 80, no associativity).
+  Reserved Notation "⧼ π , ψ , ϵ , s ⧽ ⇓ₛ ⧼ Ψ' , ϵ' , sig ⧽" (at level 80, no associativity).
 
   Declare Scope dynamics_scope.
 
-  Inductive eval (ψ : RegisterFile.t π) (ϵ : states) : Stmt.t Ω π → RegisterFile.t π → states → signal → Prop :=
+  Inductive eval (π : Π) (ψ : stringmap Value.t) (ϵ : states Π Ω) : Stmt.t Π Ω → stringmap Value.t → states Π Ω → signal → Prop :=
+    | eval_skip : ⧼ π , ψ , ϵ , Skip ⧽ ⇓ₛ ⧼ ψ , ϵ , Continue ⧽
     | eval_seq_return s₁ s₂ ψ₁ ϵ₁ v : 
-      ⧼ ψ , ϵ , s₁ ⧽ ⇓ₛ ⧼ ψ₁ , ϵ₁ , Return v ⧽ →
-      ⧼ ψ , ϵ , Seq s₁ s₂ ⧽ ⇓ₛ ⧼ ψ₁ , ϵ₁ , Return v ⧽
+      ⧼ π , ψ , ϵ , s₁ ⧽ ⇓ₛ ⧼ ψ₁ , ϵ₁ , Return v ⧽ →
+      ⧼ π , ψ , ϵ , Seq s₁ s₂ ⧽ ⇓ₛ ⧼ ψ₁ , ϵ₁ , Return v ⧽
     | eval_seq_goto s₁ s₂ ψ₁ ϵ₁ n : 
-      ⧼ ψ , ϵ , s₁ ⧽ ⇓ₛ ⧼ ψ₁ , ϵ₁ , Goto n ⧽ →
-      ⧼ ψ , ϵ , Seq s₁ s₂ ⧽ ⇓ₛ ⧼ ψ₁ , ϵ₁ , Goto n ⧽
+      ⧼ π , ψ , ϵ , s₁ ⧽ ⇓ₛ ⧼ ψ₁ , ϵ₁ , Goto n ⧽ →
+      ⧼ π , ψ , ϵ , Seq s₁ s₂ ⧽ ⇓ₛ ⧼ ψ₁ , ϵ₁ , Goto n ⧽
     | eval_seq_cont s₁ s₂ ϵ₁ ψ₁ ϵ₂ ψ₂ sig :
-      ⧼ ψ , ϵ , s₁ ⧽ ⇓ₛ ⧼ ψ₁ , ϵ₁ , Continue ⧽ →
-      ⧼ ψ₁ , ϵ₁ , s₂ ⧽ ⇓ₛ ⧼ ψ₂ , ϵ₂ , sig ⧽ →
-      ⧼ ψ , ϵ , Seq s₁ s₂ ⧽ ⇓ₛ ⧼ ψ₂ , ϵ₂ , sig ⧽
+      ⧼ π , ψ , ϵ , s₁ ⧽ ⇓ₛ ⧼ ψ₁ , ϵ₁ , Continue ⧽ →
+      ⧼ π , ψ₁ , ϵ₁ , s₂ ⧽ ⇓ₛ ⧼ ψ₂ , ϵ₂ , sig ⧽ →
+      ⧼ π , ψ , ϵ , Seq s₁ s₂ ⧽ ⇓ₛ ⧼ ψ₂ , ϵ₂ , sig ⧽
     | eval_if_true e s₁ s₂ ϵ' ϵ₁ ψ₁ sig :
-      Term.eval ψ ϵ e ϵ' true →
-      ⧼ ψ , ϵ' , s₁ ⧽ ⇓ₛ ⧼ ψ₁ , ϵ₁ , sig ⧽ →
-      ⧼ ψ , ϵ , If e s₁ s₂ ⧽ ⇓ₛ ⧼ ψ₁ , ϵ₁ , sig ⧽
+      Term.eval π ψ ϵ e ϵ' true →
+      ⧼ π , ψ , ϵ' , s₁ ⧽ ⇓ₛ ⧼ ψ₁ , ϵ₁ , sig ⧽ →
+      ⧼ π , ψ , ϵ , If e s₁ s₂ ⧽ ⇓ₛ ⧼ ψ₁ , ϵ₁ , sig ⧽
     | eval_if_false e s₁ s₂ ϵ' ϵ₂ ψ₂ sig :
-      Term.eval ψ ϵ e ϵ' false →
-      ⧼ ψ , ϵ' , s₂ ⧽ ⇓ₛ ⧼ ψ₂ , ϵ₂ , sig ⧽ →
-      ⧼ ψ , ϵ , If e s₁ s₂ ⧽ ⇓ₛ ⧼ ψ₂ , ϵ₂ , sig ⧽
+      Term.eval π ψ ϵ e ϵ' false →
+      ⧼ π , ψ , ϵ' , s₂ ⧽ ⇓ₛ ⧼ ψ₂ , ϵ₂ , sig ⧽ →
+      ⧼ π , ψ , ϵ , If e s₁ s₂ ⧽ ⇓ₛ ⧼ ψ₂ , ϵ₂ , sig ⧽
     | eval_assign x e ϵ' v :
-      Term.eval ψ ϵ e ϵ' v →
-      ⧼ ψ , ϵ , Assign x e ⧽ ⇓ₛ ⧼ <[x:=v]>ψ , ϵ , Continue ⧽
+      Term.eval π ψ ϵ e ϵ' v →
+      ⧼ π , ψ , ϵ , Assign x e ⧽ ⇓ₛ ⧼ <[x:=v]>ψ , ϵ , Continue ⧽
     | eval_goto n :
-      ⧼ ψ , ϵ , Stmt.Goto n ⧽ ⇓ₛ ⧼ ψ , ϵ , Goto n ⧽
+      ⧼ π , ψ , ϵ , Stmt.Goto n ⧽ ⇓ₛ ⧼ ψ , ϵ , Goto n ⧽
     | eval_invoke ω op arg ϵ' v :
-      Term.eval ψ ϵ (Term.Invoke ω op arg) ϵ' v →
-      ⧼ ψ , ϵ , Invoke ω op arg ⧽ ⇓ₛ ⧼ ψ , ϵ' , Continue ⧽
+      Term.eval π ψ ϵ (Term.Invoke ω op arg) ϵ' v →
+      ⧼ π , ψ , ϵ , Invoke (Invocation ω op arg) ⧽ ⇓ₛ ⧼ ψ , ϵ' , Continue ⧽
     | eval_return e ϵ' v :
-      Term.eval ψ ϵ e ϵ' v →
-      ⧼ ψ , ϵ , Stmt.Return e ⧽ ⇓ₛ ⧼ ψ , ϵ' , Return v ⧽
-  where "⧼ ψ , ϵ , s ⧽ ⇓ₛ ⧼ ψ' , ϵ' , sig ⧽" := (eval ψ ϵ s ψ' ϵ' sig) : dynamics_scope.
+      Term.eval π ψ ϵ e ϵ' v →
+      ⧼ π , ψ , ϵ , Stmt.Return e ⧽ ⇓ₛ ⧼ ψ , ϵ' , Return v ⧽
+  where "⧼ π , ψ , ϵ , s ⧽ ⇓ₛ ⧼ ψ' , ϵ' , sig ⧽" := (eval π ψ ϵ s ψ' ϵ' sig) : dynamics_scope.
 End Eval.
