theories/Dynamics/Term.v
@@ -1,21 +1,97 @@
 From Metaconfigurations Require Import 
-  Map Syntax.Term Syntax.Ty Syntax.Value Statics.Value Object Process.
-From stdpp Require Import base.
+  Map Syntax.Term Syntax.Value Object.
+From stdpp Require Import base stringmap decidable.
 Require Import Coq.ZArith.BinInt.
+Require Import Coq.Logic.FunctionalExtensionality.
+Require Import Coq.Program.Equality.
 
 Global Declare Scope dynamics_scope.
 
+Definition states (Π Ω : Type) `{Object Π Ω} := Map.dependent Ω (Σ Π ∘ type).
+
+Section DisjointUnion.
+
+  Context {Π Ω Ω' : Type}.
+
+  Context `{EqDecision Ω, Object Π Ω, EqDecision Ω', Object Π Ω'}.
+
+  Definition disjoint_union (ϵ : states Π Ω) (ϵ' : states Π Ω') : states Π (Ω + Ω') :=
+    λ ω,
+      match ω with
+      | inl ω => ϵ ω
+      | inr ω => ϵ' ω
+      end.
+
+  Notation "ϵ ⊎ ϵ'" := (disjoint_union ϵ ϵ').
+
+  Lemma rebind_union_distr ω σ ϵ ϵ' : rebind ω σ ϵ ⊎ ϵ' = rebind (inl ω) σ (ϵ ⊎ ϵ').
+  Proof.
+    extensionality ω'. destruct ω'.
+    - simpl. unfold rebind, disjoint_union. case_decide.
+      + destruct H1. case_decide.
+        * dependent destruction H1. reflexivity.
+        * contradiction.
+      + case_decide. 
+        * dependent destruction H2. contradiction.
+        * reflexivity.
+    - simpl. unfold rebind, disjoint_union. case_decide.
+      + dependent destruction H1.
+      + reflexivity.
+  Qed.
+
+  Lemma lookup_union_distr ω ϵ ϵ' : Map.lookup ω ϵ = Map.lookup (inl ω) (ϵ ⊎ ϵ').
+  Proof. reflexivity. Qed.
+
+  Lemma union_inj ϵ₁ ϵ₁' ϵ₂ ϵ₂' : ϵ₁ ⊎ ϵ₁' = ϵ₂ ⊎ ϵ₂' → ϵ₁ = ϵ₂ ∧ ϵ₁' = ϵ₂'.
+  Proof.
+    intros. split; extensionality ω.
+    - eapply equal_f_dep with (x := inl ω) in H1. auto. 
+    - eapply equal_f_dep with (x := inr ω) in H1. auto.
+  Qed.
+
+  Definition πₗ (ϵ : states Π (Ω + Ω')) : states Π Ω := λ ω, ϵ (inl ω).
+
+  Definition πᵣ (ϵ : states Π (Ω + Ω')) : states Π Ω' := λ ω, ϵ (inr ω).
+
+  Lemma πₗ_union ϵ₁ ϵ₂ : πₗ (ϵ₁ ⊎ ϵ₂) = ϵ₁.
+  Proof.
+    extensionality ω. reflexivity.
+  Qed.
+
+  Lemma πᵣ_union ϵ₁ ϵ₂ : πᵣ (ϵ₁ ⊎ ϵ₂) = ϵ₂.
+  Proof.
+    extensionality ω. reflexivity.
+  Qed.
+
+  Lemma union_project ϵ : πₗ ϵ ⊎ πᵣ ϵ = ϵ.
+  Proof. extensionality ω. intuition. Qed.
+
+  Lemma πₗ_rebind_comm ω σ ϵ : πₗ (rebind (inl ω) σ ϵ) = rebind ω σ (πₗ ϵ).
+  Proof.
+    intros. extensionality ω'. unfold rebind. case_decide.
+    - subst. cbv. destruct (EqDecision1 ω' ω').
+      + dependent destruction e. reflexivity.
+      + contradiction.
+    - cbv. destruct (EqDecision1 ω ω').
+      + contradiction.
+      + reflexivity.
+  Qed.
+
+  Lemma lookup_πₗ ω ϵ : Map.lookup ω (πₗ ϵ) = Map.lookup (inl ω) ϵ.
+  Proof. reflexivity. Qed.
+
+  Lemma rebind_l_πᵣ ω ϵ σ : πᵣ ϵ = πᵣ (rebind (inl ω) σ ϵ).
+  Proof. extensionality ω'. reflexivity. Qed.
+
+End DisjointUnion.
+
 Section Eval.
 
-  Context {Π : Type} `{Process Π}.
+  Context {Π : Type}.
 
   Context {Ω : Type} `{Object Π Ω}.
 
-  Context {π : Π}.
-
-  Definition states := Map.dependent Ω (Σ Π ∘ type).
-
-  Reserved Notation "⟨ Ψ , ϵ , e ⟩ ⇓ₑ ⟨ ϵ' , v ⟩" (at level 80, no associativity).
+  Reserved Notation "⟨ π , Ψ , ϵ , e ⟩ ⇓ₑ ⟨ ϵ' , v ⟩" (at level 80, no associativity).
 
   Variant eval_binop : Term.bop → Value.t → Value.t → Value.t → Set :=
     | eval_add (n₁ n₂ : Z) : eval_binop Term.Add n₁ n₂ (n₁ + n₂)%Z
@@ -36,44 +112,43 @@ Section Eval.
 
 (* (ω : Ω) (op : (type ω).(OP Π)) (arg : (type ω).(ARG Π) *)
 
-  Variant eval_inv ϵ ω op arg σ res :=
+  Variant eval_inv π ϵ ω op arg σ res :=
     | eval_inv_intro :
-      ∀ H : ⊢ᵥ arg `: (type ω).(ARG Π) op,
-      (type ω).(δ Π) (Map.lookup ω ϵ) π op (exist _ arg H) = (σ, res) →
-      eval_inv ϵ ω op arg σ res.
+      (type ω).(δ Π) (Map.lookup ω ϵ) π op arg σ res →
+      eval_inv π ϵ ω op arg σ res.
 
-  Inductive eval (ψ : RegisterFile.t π) (ϵ : states) : Term.t Ω π → states → Value.t → Prop := 
+  Inductive eval (π : Π) (ψ : stringmap Value.t) (ϵ : states Π Ω) : Term.t Π Ω → states Π Ω → Value.t → Prop := 
     | eval_var x v :
       ψ !! x = Some v →
-      ⟨ ψ , ϵ , Reg x ⟩ ⇓ₑ ⟨ ϵ , v ⟩
+      ⟨ π , ψ , ϵ , Var x ⟩ ⇓ₑ ⟨ ϵ , v ⟩
     | eval_invoke ω op arg argᵥ res ϵ' σ :
-      ⟨ ψ , ϵ , arg ⟩ ⇓ₑ ⟨ ϵ' , argᵥ ⟩ →
-      eval_inv ϵ ω op argᵥ σ res →
-      ⟨ ψ , ϵ , Invoke ω op arg ⟩ ⇓ₑ ⟨ rebind ω σ ϵ' , proj1_sig res ⟩
+      ⟨ π , ψ , ϵ , arg ⟩ ⇓ₑ ⟨ ϵ' , argᵥ ⟩ →
+      eval_inv π ϵ ω op argᵥ σ res →
+      ⟨ π , ψ , ϵ , Invoke ω op arg ⟩ ⇓ₑ ⟨ rebind ω σ ϵ' , res ⟩
     | eval_bop bop e₁ e₂ v₁ v₂ v ϵ₁ ϵ₂ : 
-      ⟨ ψ , ϵ , e₁ ⟩ ⇓ₑ ⟨ ϵ₁ , v₁ ⟩ →
-      ⟨ ψ , ϵ₁ , e₂ ⟩ ⇓ₑ ⟨ ϵ₂ , v₂ ⟩ →
+      ⟨ π , ψ , ϵ , e₁ ⟩ ⇓ₑ ⟨ ϵ₁ , v₁ ⟩ →
+      ⟨ π , ψ , ϵ₁ , e₂ ⟩ ⇓ₑ ⟨ ϵ₂ , v₂ ⟩ →
       eval_binop bop v₁ v₂ v →
-      ⟨ ψ , ϵ , Bop bop e₁ e₂ ⟩ ⇓ₑ ⟨ ϵ₂ , v ⟩
+      ⟨ π , ψ , ϵ , Bop bop e₁ e₂ ⟩ ⇓ₑ ⟨ ϵ₂ , v ⟩
     | eval_uop e uop ϵ' v v' :
-      ⟨ ψ , ϵ , e ⟩ ⇓ₑ ⟨ ϵ' , v ⟩ →
+      ⟨ π , ψ , ϵ , e ⟩ ⇓ₑ ⟨ ϵ' , v ⟩ →
       eval_unop uop v v' → 
-      ⟨ ψ , ϵ , Uop uop e ⟩ ⇓ₑ ⟨ ϵ' , v' ⟩
+      ⟨ π , ψ , ϵ , Uop uop e ⟩ ⇓ₑ ⟨ ϵ' , v' ⟩
     | eval_pair e₁ e₂ v₁ v₂ ϵ₁ ϵ₂ :
-      ⟨ ψ , ϵ , e₁ ⟩ ⇓ₑ ⟨ ϵ₁ , v₁ ⟩ →
-      ⟨ ψ , ϵ₁ , e₂ ⟩ ⇓ₑ ⟨ ϵ₂ , v₂ ⟩ →
-      ⟨ ψ , ϵ , Term.Pair e₁ e₂ ⟩ ⇓ₑ ⟨ ϵ₂ , Pair v₁ v₂ ⟩
+      ⟨ π , ψ , ϵ , e₁ ⟩ ⇓ₑ ⟨ ϵ₁ , v₁ ⟩ →
+      ⟨ π , ψ , ϵ₁ , e₂ ⟩ ⇓ₑ ⟨ ϵ₂ , v₂ ⟩ →
+      ⟨ π , ψ , ϵ , Term.Pair e₁ e₂ ⟩ ⇓ₑ ⟨ ϵ₂ , Pair v₁ v₂ ⟩
     | eval_projl e v₁ v₂ ϵ' :
-      ⟨ ψ , ϵ , e ⟩ ⇓ₑ ⟨ ϵ' , Pair v₁ v₂ ⟩ →
-      ⟨ ψ , ϵ , ProjL e ⟩ ⇓ₑ ⟨ ϵ' , v₁ ⟩
+      ⟨ π , ψ , ϵ , e ⟩ ⇓ₑ ⟨ ϵ' , Pair v₁ v₂ ⟩ →
+      ⟨ π , ψ , ϵ , ProjL e ⟩ ⇓ₑ ⟨ ϵ' , v₁ ⟩
     | eval_projr e v₁ v₂ ϵ' :
-      ⟨ ψ , ϵ , e ⟩ ⇓ₑ ⟨ ϵ' , Pair v₁ v₂ ⟩ →
-      ⟨ ψ , ϵ , ProjR e ⟩ ⇓ₑ ⟨ ϵ' , v₂ ⟩
+      ⟨ π , ψ , ϵ , e ⟩ ⇓ₑ ⟨ ϵ' , Pair v₁ v₂ ⟩ →
+      ⟨ π , ψ , ϵ , ProjR e ⟩ ⇓ₑ ⟨ ϵ' , v₂ ⟩
     | eval_int n :
-      ⟨ ψ , ϵ , Term.Int n ⟩ ⇓ₑ ⟨ ϵ , n ⟩
+      ⟨ π , ψ , ϵ , Term.Int n ⟩ ⇓ₑ ⟨ ϵ , n ⟩
     | eval_bool b :
-      ⟨ ψ , ϵ , Term.Bool b ⟩ ⇓ₑ ⟨ ϵ , b ⟩
+      ⟨ π , ψ , ϵ , Term.Bool b ⟩ ⇓ₑ ⟨ ϵ , b ⟩
     | eval_unit :
-      ⟨ ψ , ϵ , ⊤ₑ ⟩ ⇓ₑ ⟨ ϵ , ⊤ᵥ ⟩
-  where "⟨ ψ , ϵ , e ⟩ ⇓ₑ ⟨ ϵ' , v ⟩" := (eval ψ ϵ e ϵ' v) : dynamics_scope.
+      ⟨ π , ψ , ϵ , ⊤ₑ ⟩ ⇓ₑ ⟨ ϵ , ⊤ᵥ ⟩
+  where "⟨ π , ψ , ϵ , e ⟩ ⇓ₑ ⟨ ϵ' , v ⟩" := (eval π ψ ϵ e ϵ' v) : dynamics_scope.
 End Eval.
