theories/Object.v
@@ -1,19 +1,24 @@
 From stdpp Require Import base gmap.
 Require Import Coq.Sets.Ensembles.
 Require Import Coq.Strings.String.
-From Metaconfigurations.Syntax Require Import Value Ty.
-From Metaconfigurations.Statics Require Import Value.
+From Metaconfigurations.Syntax Require Import Value.
 
 Record object_type (Π : Type) := {
   Σ : Type;
   OP : Type;
-  (* OP : ARG OP → RES OP *)
-  ARG : OP → Ty.t;
-  RES : OP → Ty.t;
-  δ : Σ → Π → ∀ op, V⟦ ARG op ⟧ → Σ * V⟦ RES op ⟧;
+  δ : Σ → Π → OP → Value.t → Σ → Value.t → Prop;
 }.
 
 Class Object (Π : Type) (Ω : Type) `{EqDecision Ω} := {
   type : Ω → object_type Π;
   (* state : ∀ (ω : Ω), (type ω).(Σ Π) *)
 }.
+
+Instance augmentation_Object (Ω Ω' Π : Type) `{Object Π Ω, Object Π Ω'} : Object Π (Ω + Ω') := {
+  type obj :=
+    match obj with
+    | inl ω => type ω
+    | inr ω => type ω
+    end
+}.
+
