theories/Syntax/Stmt.v
@@ -1,33 +1,31 @@
 From stdpp Require Import base gmap.
-From Metaconfigurations Require Import Syntax.Term Object Process.
+From Metaconfigurations Require Import Syntax.Term Object.
 Require Import Coq.Strings.String.
 
 Section Stmt.
 
-  Context {Π : Type} `{Process Π}.
-
-  Variable Ω : Type.
+  Variables Π Ω : Type.
 
   Context `{Object Π Ω}.
 
-  Variable π : Π.
-
   Inductive t : Type :=
     | Seq (s₁ : t) (s₂ : t)
-    | Assign (x : register_names π) (e : Term.t Ω π)
-    | If (e : Term.t Ω π) (s₁ : t) (s₂ : t)
+    | Assign (x : string) (e : Term.t Π Ω)
+    | If (e : Term.t Π Ω) (s₁ : t) (s₂ : t)
     | Goto (l : nat)
-    | Return (e : Term.t Ω π)
-    | Invoke (ω : Ω) (op : (type ω).(OP Π)) (arg : Term.t Ω π).
+    | Return (e : Term.t Π Ω)
+    | Invoke (inv : invocation Π Ω)
+    | Skip.
 
   Notation "s₁ `; s₂" := (Seq s₁ s₂) (at level 80).
   Notation "x ← e" := (Assign x e) (at level 80).
 
 End Stmt.
 
-Arguments Seq {_ _ _ _ _ _}.
-Arguments Assign {_ _ _ _ _ _}.
-Arguments If {_ _ _ _ _ _ }.
-Arguments Goto {_ _ _ _ _ _}.
-Arguments Return {_ _ _ _ _ _}.
-Arguments Invoke {_ _ _ _ _ _}.
+Arguments Seq {_ _ _ _}.
+Arguments Assign {_ _ _ _}.
+Arguments If {_ _ _ _}.
+Arguments Goto {_ _ _ _}.
+Arguments Return {_ _ _ _}.
+Arguments Invoke {_ _ _ _}.
+Arguments Skip {_ _ _ _}.
