theories/Syntax/Term.v
@@ -1,7 +1,7 @@
 From stdpp Require Import base gmap.
 Require Import Coq.Strings.String.
 Require Import Coq.Lists.List.
-From Metaconfigurations Require Import Object Process.
+From Metaconfigurations Require Import Object.
 
 Variant bop : Set :=
   | Add
@@ -14,28 +14,39 @@ Variant uop : Set := Not.
 
 Declare Scope term_scope.
 
-Inductive t {Π : Type} (Ω : Type) (π : Π) `{Process Π} `{Object Π Ω} : Type :=
-  | Reg (x : register_names π)
-  | Invoke (ω : Ω) (op : (type ω).(OP Π)) (arg : t Ω π)
-  | Bop (op : bop) (e₁ : t Ω π) (e₂ : t Ω π)
-  | Uop (op : uop) (e : t Ω π)
-  | Pair (e₁ : t Ω π) (e₂ : t Ω π)
-  | ProjL (e : t Ω π)
-  | ProjR (e : t Ω π)
-  | Int (n : Z)
-  | Bool (b : bool)
-  | Unit.
+Section Term.
 
-Arguments Reg {Π Ω π _ _ _}.
-Arguments Invoke {Π Ω π _ _ _}.
-Arguments Bop {Π Ω π _ _ _}.
-Arguments Uop {Π Ω π _ _ _}.
-Arguments Pair {Π Ω π _ _ _}.
-Arguments ProjL {Π Ω π _ _ _}.
-Arguments ProjR {Π Ω π _ _ _}.
-Arguments Int {Π Ω π _ _ _}.
-Arguments Bool {Π Ω π _ _ _}.
-Arguments Unit {Π Ω π _ _ _}.
+  Variables Π Ω : Type.
+
+  Context `{Object Π Ω}.
+
+  Inductive t : Type :=
+    | Var (x : string)
+    | Invoke (ω : Ω) (op : (type ω).(OP Π)) (arg : t)
+    | Bop (op : bop) (e₁ : t) (e₂ : t)
+    | Uop (op : uop) (e : t)
+    | Pair (e₁ : t) (e₂ : t)
+    | ProjL (e : t)
+    | ProjR (e : t)
+    | Int (n : Z)
+    | Bool (b : bool)
+    | Unit.
+
+  Variant invocation : Type := Invocation (ω : Ω) (op : (type ω).(OP Π)) (arg : t).
+
+End Term.
+
+Arguments Var {Π Ω _ _}.
+Arguments Invoke {Π Ω _ _}.
+Arguments Bop {Π Ω _ _}.
+Arguments Uop {Π Ω _ _}.
+Arguments Pair {Π Ω _ _}.
+Arguments ProjL {Π Ω _ _}.
+Arguments ProjR {Π Ω _ _}.
+Arguments Int {Π Ω _ _}.
+Arguments Bool {Π Ω _ _}.
+Arguments Unit {Π Ω _ _}.
+Arguments Invocation {_ _ _ _}.
 
 Notation "'⊤ₑ'" := Unit.
 
