theories/Syntax/Value.v
@@ -1,5 +1,4 @@
 From stdpp Require Import base gmap.
-Require Import Metaconfigurations.Syntax.Ty.
 Require Import Coq.Classes.SetoidDec.
 Require Import Coq.ZArith.BinInt.
 Require Import Coq.Lists.List.
